src/Soundness.v
@@ -68,14 +68,14 @@ Module Soundness (P : PAT).
       forwards [ k [ Heq Hle ] ] : Nat.lt_exists_pred x y ; subst ; rew_nat*.
     Qed.
 
-    Lemma tm_subst_fresh : forall t x u, var_fresh x t -> tm_subst t x u = t.
+    Lemma tm_fsubst_fresh : forall t x u, var_fresh x t -> tm_fsubst t x u = t.
     Proof.
       introv Hfresh. unfolds.
       induction* t ; fequals ; try (injection Hfresh ; auto_star).
       { Case "TmFVar". cases_if*. lets* ? : var_not_fresh v. }
     Qed.
 
-    Lemma ty_subst_fresh : forall t x u, tvar_fresh x t -> ty_subst t x u = t.
+    Lemma ty_fsubst_fresh : forall t x u, tvar_fresh x t -> ty_fsubst t x u = t.
     Proof.
       introv Hfresh. unfolds.
       induction* t ; fequals ; try (injection Hfresh ; auto_star).
@@ -109,37 +109,37 @@ Module Soundness (P : PAT).
       forall ty x y,
         x <= y ->
         tm_freshen (tm_defreshen ty y) x = tm_defreshen (tm_freshen ty x) (S y).
-    Proof. magic ty ; nat_math. Qed.
+    Proof. magic ty. Qed.
 
     Lemma ty_freshen_defreshen :
       forall ty x y,
         x <= y ->
         ty_freshen (ty_defreshen ty y) x = ty_defreshen (ty_freshen ty x) (S y).
-    Proof. magic ty ; nat_math. Qed.
+    Proof. magic ty. Qed.
 
     Lemma tm_ty_freshen_defreshen :
       forall ty x y,
         tm_ty_freshen (tm_defreshen ty y) x = tm_defreshen (tm_ty_freshen ty x) y.
     Proof. magic ty. Qed.
 
-    Lemma tm_freshen_subst :
+    Lemma tm_freshen_fsubst :
       forall t x y u,
         x <= y ->
-        tm_freshen (tm_subst t y u) x =
-          tm_subst (tm_freshen t x) (S y) (tm_freshen u x).
+        tm_freshen (tm_fsubst t y u) x =
+          tm_fsubst (tm_freshen t x) (S y) (tm_freshen u x).
     Proof. magic t. Qed.
 
-    Lemma ty_freshen_subst :
+    Lemma ty_freshen_fsubst :
       forall t x y u,
         x <= y ->
-        ty_freshen (ty_subst t y u) x =
-          ty_subst (ty_freshen t x) (S y) (ty_freshen u x).
+        ty_freshen (ty_fsubst t y u) x =
+          ty_fsubst (ty_freshen t x) (S y) (ty_freshen u x).
     Proof. magic t. Qed.
 
-    Lemma tm_ty_freshen_subst :
+    Lemma tm_ty_freshen_fsubst :
       forall t x y u,
-        tm_ty_freshen (tm_subst t y u) x =
-          tm_subst (tm_ty_freshen t x) y (tm_ty_freshen u x).
+        tm_ty_freshen (tm_fsubst t y u) x =
+          tm_fsubst (tm_ty_freshen t x) y (tm_ty_freshen u x).
     Proof. magic t. Qed.
 
     Lemma tm_freshen_bsubst : forall t y z u,
@@ -235,175 +235,177 @@ Module Soundness (P : PAT).
         rewrite Hfv. rewrite* <- ty_defreshen_bsubst. }
     Qed.
 
-    (* TODO: can freshen be separated out from these lemmas into separate ones? *)
-    Lemma ty_bsubst_neq : forall ty x y ty1 ty2,
-        x <> y ->
-        ty_bsubst (ty_bsubst (ty_freshen ty 0) x ty1) y ty2 = ty_bsubst (ty_freshen ty 0) x ty1 ->
+    (* TODO: These lemmas can be stated in terms of bsubst only, e.g., *)
+    (*  x <> y ->
+        ty_bsubst (ty_bsubst ty x ty1) y ty2 = ty_bsubst ty x ty1 ->
         ty_bsubst ty y ty2 = ty.
-    Proof. magic ty ; with_hyp (_ = _) as Heq ; inverts* Heq. Qed.
-
-    Lemma tm_bsubst_neq : forall t x y u1 u2,
+     *)
+    (* Can we separate out the open/freshen part in a good way? *)
+    Lemma ty_bsubst_neq : forall ty x y z ty',
         x <> y ->
-        tm_bsubst (tm_bsubst (tm_freshen t 0) x u1) y u2 = tm_bsubst (tm_freshen t 0) x u1 ->
-        tm_bsubst t y u2 = t.
-    Proof. magic t ; with_hyp (_ = _) as Heq ; inverts* Heq. Qed.
+        ty_bsubst (ty_open ty x z) y ty' = ty_open ty x z ->
+        ty_bsubst ty y ty' = ty.
+    Proof. unfolds ty_open ; magic ty ; with_hyp (_ = _) as Heq ; inverts* Heq. Qed.
 
-    Lemma tm_ty_bsubst_neq : forall t x y ty1 ty2,
+    Lemma tm_bsubst_neq : forall t x y z u,
         x <> y ->
-        tm_ty_bsubst (tm_ty_bsubst (tm_ty_freshen t 0) x ty1) y ty2 =
-          tm_ty_bsubst (tm_ty_freshen t 0) x ty1 ->
-        tm_ty_bsubst t y ty2 = t.
+        tm_bsubst (tm_open t x z) y u = tm_open t x z ->
+        tm_bsubst t y u = t.
+    Proof. unfolds tm_open ; magic t ; with_hyp (_ = _) as Heq ; inverts* Heq. Qed.
+
+    Lemma tm_ty_bsubst_neq : forall t x y z ty,
+        x <> y ->
+        tm_ty_bsubst (tm_ty_open t x z) y ty = tm_ty_open t x z ->
+        tm_ty_bsubst t y ty = t.
     Proof.
       introv Hneq Heq ; gen x y ; magic t ; inverts* Heq ;
         with_hyp (ty_bsubst _ _ _ = _) as Heq1 ; applys ty_bsubst_neq Hneq Heq1.
     Qed.
 
-    Lemma tm_bsubst_ty_rec : forall t x y ty u,
-        tm_bsubst (tm_ty_bsubst (tm_ty_freshen t 0) x ty) y u =
-          tm_ty_bsubst (tm_ty_freshen t 0) x ty ->
+    Lemma tm_bsubst_ty_rec : forall t x y z u,
+        tm_bsubst (tm_ty_open t x z) y u = tm_ty_open t x z ->
         tm_bsubst t y u = t.
     Proof. magic t ; with_hyp (_ = _) as Heq ; inverts* Heq. Qed.
 
-    Lemma tm_ty_bsubst_rec : forall t x y ty u,
-        tm_ty_bsubst (tm_bsubst (tm_freshen t 0) x u) y ty =
-          tm_bsubst (tm_freshen t 0) x u ->
+    Lemma tm_ty_bsubst_rec : forall t x y z ty,
+        tm_ty_bsubst (tm_open t x z) y ty = tm_open t x z ->
         tm_ty_bsubst t y ty = t.
-    Proof. magic t ; with_hyp (_ = _) as Heq ; inverts* Heq. Qed.
+    Proof. unfolds tm_open ; magic t ; with_hyp (_ = _) as Heq ; inverts* Heq. Qed.
 
     Lemma tm_bsubst_lc : forall t y u, tm_lc t -> tm_bsubst t y u = t.
     Proof.
       introv Hlc. gen y.
       induction Hlc ; intros ; simpls ; fequals*.
-      { Case "TmLam". rewrite tm_bsubst_neq with (x := 0) (u1 := TmFVar 0) ; auto. }
-      { Case "TmTyLam". rewrite tm_bsubst_ty_rec with (x := 0) (ty := TyFVar 0) ; auto. }
+      { Case "TmLam". rewrite tm_bsubst_neq with (x := 0) (z := 0) ; auto. }
+      { Case "TmTyLam". rewrite tm_bsubst_ty_rec with (x := 0) (z := 0) ; auto. }
     Qed.
 
     Lemma ty_bsubst_lc : forall ty y u, ty_lc ty -> ty_bsubst ty y u = ty.
     Proof.
       introv Hlc. gen y.
       induction Hlc ; intros ; simpls ; fequals*.
-      { Case "TyAll". rewrite ty_bsubst_neq with (x := 0) (ty1 := TyFVar 0) ; auto. }
+      { Case "TyAll". rewrite ty_bsubst_neq with (x := 0) (z := 0) ; auto. }
     Qed.
 
     Lemma tm_ty_bsubst_lc : forall t y ty, tm_lc t -> tm_ty_bsubst t y ty = t.
     Proof.
       introv Hlc. gen y.
       induction Hlc ; intros ; simpls ; fequals* ; try apply* ty_bsubst_lc.
-      { Case "TmLam". rewrite tm_ty_bsubst_rec with (x := 0) (u := TmFVar 0) ; auto. }
-      { Case "TmTyLam". rewrite tm_ty_bsubst_neq with (x := 0) (ty1 := TyFVar 0) ; auto. }
+      { Case "TmLam". rewrite tm_ty_bsubst_rec with (x := 0) (z := 0) ; auto. }
+      { Case "TmTyLam". rewrite tm_ty_bsubst_neq with (x := 0) (z := 0) ; auto. }
     Qed.
 
-    Lemma tm_subst_bsubst_distr :
+    Lemma tm_fsubst_bsubst_distr :
       forall t x y u1 u2,
         tm_lc u1 ->
-        tm_subst (tm_bsubst t y u2) x u1 =
-          tm_bsubst (tm_subst t x u1) y (tm_subst u2 x u1).
+        tm_fsubst (tm_bsubst t y u2) x u1 =
+          tm_bsubst (tm_fsubst t x u1) y (tm_fsubst u2 x u1).
     Proof. magic t ; rewrite* tm_bsubst_lc. Qed.
 
-    Lemma ty_subst_bsubst_distr :
+    Lemma ty_fsubst_bsubst_distr :
       forall t x y u1 u2,
         ty_lc u1 ->
-        ty_subst (ty_bsubst t y u2) x u1 =
-          ty_bsubst (ty_subst t x u1) y (ty_subst u2 x u1).
+        ty_fsubst (ty_bsubst t y u2) x u1 =
+          ty_bsubst (ty_fsubst t x u1) y (ty_fsubst u2 x u1).
     Proof. magic t ; rewrite* ty_bsubst_lc. Qed.
 
-    Lemma tm_subst_intro :
+    Lemma tm_fsubst_intro :
       forall t x y u,
         var_fresh x t ->
-        tm_bsubst t y u = tm_subst (tm_bsubst t y (TmFVar x)) x u.
+        tm_bsubst t y u = tm_fsubst (tm_bsubst t y (TmFVar x)) x u.
     Proof.
       introv Hfresh ; gen y ; magic t ; try (injection Hfresh ; auto_star).
       { Case "TmFVar". subst. lets* ? : var_not_fresh v. }
     Qed.
 
-    Lemma ty_subst_intro :
+    Lemma ty_fsubst_intro :
       forall x y ty u,
         tvar_fresh x ty ->
-        ty_bsubst ty y u = ty_subst (ty_bsubst ty y (TyFVar x)) x u.
+        ty_bsubst ty y u = ty_fsubst (ty_bsubst ty y (TyFVar x)) x u.
     Proof.
       introv Hfresh ; gen y ; magic ty ; try (injection Hfresh ; auto_star).
       { Case "TmFVar". subst. lets* ? : tvar_not_fresh t. }
     Qed.
 
-    Lemma tm_subst_open :
-      forall t u,
-        tm_bsubst t 0 u = tm_defreshen (tm_subst (tm_open t) 0 (tm_freshen u 0)) 0.
+    Lemma tm_bsubst_close_open :
+      forall t u x y,
+        tm_bsubst t y u = tm_close (tm_open t y x) x u.
     Proof.
       intros.
-      rewrite <- tm_defreshen_freshen with (x := 0) (t := tm_bsubst t 0 u).
-      rewrite tm_freshen_bsubst. rewrite tm_subst_intro with (x := 0) ; auto. apply tm_freshen_fresh.
+      rewrite <- tm_defreshen_freshen with (x := x) (t := tm_bsubst t y u).
+      rewrite tm_freshen_bsubst. rewrite tm_fsubst_intro with (x := x) ; auto. apply tm_freshen_fresh.
     Qed.
 
-    Lemma ty_subst_open :
-      forall ty u,
-        ty_bsubst ty 0 u = ty_defreshen (ty_subst (ty_open ty) 0 (ty_freshen u 0)) 0.
+    Lemma ty_bsubst_close_open :
+      forall ty u x y,
+        ty_bsubst ty y u = ty_close (ty_open ty y x) x u.
     Proof.
       intros.
-      rewrite <- ty_defreshen_freshen with (x := 0) (t := ty_bsubst ty 0 u).
-      rewrite ty_freshen_bsubst. rewrite ty_subst_intro with (x := 0) ; auto. apply ty_freshen_fresh.
+      rewrite <- ty_defreshen_freshen with (x := x) (t := ty_bsubst ty y u).
+      rewrite ty_freshen_bsubst. rewrite ty_fsubst_intro with (x := x) ; auto. apply ty_freshen_fresh.
     Qed.
 
-    Lemma tm_bsubst_subst_comm :
+    Lemma tm_bsubst_fsubst_comm :
       forall t x y z u,
         x <> z ->
         tm_lc u ->
-        tm_bsubst (tm_subst t x u) y (TmFVar z) =
-          tm_subst (tm_bsubst t y (TmFVar z)) x u.
+        tm_bsubst (tm_fsubst t x u) y (TmFVar z) =
+          tm_fsubst (tm_bsubst t y (TmFVar z)) x u.
     Proof.
       introv Hneq Hlc. symmetry.
-      applys_eq* tm_subst_bsubst_distr. fequals.
-      rewrite* tm_subst_fresh. apply* var_neq_fresh.
+      applys_eq* tm_fsubst_bsubst_distr. fequals.
+      rewrite* tm_fsubst_fresh. apply* var_neq_fresh.
     Qed.
 
-    Lemma ty_bsubst_subst_comm :
+    Lemma ty_bsubst_fsubst_comm :
       forall t x y z u,
         x <> z ->
         ty_lc u ->
-        ty_bsubst (ty_subst t x u) y (TyFVar z) =
-          ty_subst (ty_bsubst t y (TyFVar z)) x u.
+        ty_bsubst (ty_fsubst t x u) y (TyFVar z) =
+          ty_fsubst (ty_bsubst t y (TyFVar z)) x u.
     Proof.
       introv Hneq Hlc. symmetry.
-      applys_eq* ty_subst_bsubst_distr. fequals.
-      rewrite* ty_subst_fresh. apply* tvar_neq_fresh.
+      applys_eq* ty_fsubst_bsubst_distr. fequals.
+      rewrite* ty_fsubst_fresh. apply* tvar_neq_fresh.
     Qed.
 
-    Lemma tm_ty_bsubst_subst_comm :
+    Lemma tm_ty_bsubst_fsubst_comm :
       forall t x y u ty,
         tm_lc u ->
-        tm_ty_bsubst (tm_subst t x u) y ty =
-          tm_subst (tm_ty_bsubst t y ty) x u.
+        tm_ty_bsubst (tm_fsubst t x u) y ty =
+          tm_fsubst (tm_ty_bsubst t y ty) x u.
     Proof. magic t ; rewrite* tm_ty_bsubst_lc. Qed.
 
-    Lemma tm_open_subst_comm :
-      forall t x u,
+    Lemma tm_open_fsubst_comm :
+      forall t x y u,
         tm_lc u ->
-        tm_open (tm_subst t x u) = tm_subst (tm_open t) (S x) (tm_freshen u 0).
+        tm_open (tm_fsubst t x u) y 0 = tm_fsubst (tm_open t y 0) (S x) (tm_freshen u 0).
     Proof.
-      introv Hlc. unfolds. rewrite tm_freshen_subst. applys* tm_bsubst_subst_comm.
+      introv Hlc. unfolds. rewrite tm_freshen_fsubst. applys* tm_bsubst_fsubst_comm.
       apply* tm_freshen_lc. nat_math.
     Qed.
 
-    Lemma ty_open_subst_comm :
-      forall t x u,
+    Lemma ty_open_fsubst_comm :
+      forall t x y u,
         ty_lc u ->
-        ty_open (ty_subst t x u) = ty_subst (ty_open t) (S x) (ty_freshen u 0).
+        ty_open (ty_fsubst t x u) y 0 = ty_fsubst (ty_open t y 0) (S x) (ty_freshen u 0).
     Proof.
-      introv Hlc. unfolds. rewrite ty_freshen_subst. applys* ty_bsubst_subst_comm.
+      introv Hlc. unfolds. rewrite ty_freshen_fsubst. applys* ty_bsubst_fsubst_comm.
       apply* ty_freshen_lc. nat_math.
     Qed.
 
-    Lemma tm_ty_open_subst_comm :
-      forall t x u,
+    Lemma tm_ty_open_fsubst_comm :
+      forall t x y u,
         tm_lc u ->
-        tm_ty_open (tm_subst t x u) = tm_subst (tm_ty_open t) x (tm_ty_freshen u 0).
+        tm_ty_open (tm_fsubst t x u) y 0 = tm_fsubst (tm_ty_open t y 0) x (tm_ty_freshen u 0).
     Proof.
-      introv Hlc. unfolds. rewrite tm_ty_freshen_subst. applys* tm_ty_bsubst_subst_comm.
+      introv Hlc. unfolds. rewrite tm_ty_freshen_fsubst. applys* tm_ty_bsubst_fsubst_comm.
       apply* tm_ty_freshen_lc.
     Qed.
 
     Lemma tm_open_defreshen_comm :
-      forall t x,
-        tm_open (tm_defreshen t x) = tm_defreshen (tm_open t) (S x).
+      forall t x y,
+        tm_open (tm_defreshen t x) y 0 = tm_defreshen (tm_open t y 0) (S x).
     Proof.
       intros. unfolds. rewrite tm_freshen_defreshen ; try nat_math.
       assert (Hfv : TmFVar 0 = tm_defreshen (TmFVar 0) (S x)) by simple_math.
@@ -411,23 +413,23 @@ Module Soundness (P : PAT).
     Qed.
 
     Lemma tm_ty_open_defreshen_comm :
-      forall t x,
-        tm_ty_open (tm_defreshen t x) = tm_defreshen (tm_ty_open t) x.
+      forall t x y,
+        tm_ty_open (tm_defreshen t x) y 0 = tm_defreshen (tm_ty_open t y 0) x.
     Proof.
       intros. unfolds. rewrite tm_ty_freshen_defreshen.
       rewrite* tm_defreshen_ty_bsubst.
     Qed.
 
-    Lemma ty_lc_subst :
+    Lemma ty_lc_fsubst :
       forall ty1 ty2 x,
         ty_lc ty1 ->
         ty_lc ty2 ->
-        ty_lc (ty_subst ty1 x ty2).
+        ty_lc (ty_fsubst ty1 x ty2).
     Proof.
       introv Hlc1 Hlc2. gen x ty2.
       induction* Hlc1 ; intros ; simpls*.
       { Case "TyBVar". case_if*. }
-      { Case "TyAll". constructor*. rewrite* ty_open_subst_comm.
+      { Case "TyAll". constructor*. rewrite* ty_open_fsubst_comm.
         applys* IHHlc1. apply* ty_freshen_lc. }
     Qed.
 
@@ -468,8 +470,8 @@ Module Soundness (P : PAT).
       { Case "TmApp". inverts* IHttype1. }
       { Case "TmTyApp".
         inverts* IHttype.
-        rewrite ty_subst_open.
-        apply ty_defreshen_lc. apply* ty_lc_subst. apply ty_freshen_lc. apply* ok_type_lct. }
+        rewrite ty_bsubst_close_open with (x := 0).
+        apply ty_defreshen_lc. apply* ty_lc_fsubst. apply ty_freshen_lc. apply* ok_type_lct. }
     Qed.
 
     Lemma ok_term_lc :
@@ -485,25 +487,25 @@ Module Soundness (P : PAT).
     Lemma ok_data_strengthen_var :
       forall G1 G2 ty' d,
         ok_data (G1 ++ BindVar ty' :: G2) d ->
-        ok_data (G1 ++ SkipVar :: G2) d.
+        ok_data (G1 ++ G2) d.
     Proof. Admitted.
 
     Lemma ok_kind_strengthen_var :
       forall G1 G2 ty' k,
         ok_kind (G1 ++ BindVar ty' :: G2) k ->
-        ok_kind (G1 ++ SkipVar :: G2) k.
+        ok_kind (G1 ++ G2) k.
     Proof. Admitted.
 
     Lemma ok_type_strengthen_var :
       forall G1 G2 ty' ty k,
         ok_type (G1 ++ BindVar ty' :: G2) ty k ->
-        ok_type (G1 ++ SkipVar :: G2) ty k.
+        ok_type (G1 ++ G2) ty k.
     Proof. Admitted.
 
     Lemma ok_env_strengthen_var :
       forall G1 G2 ty,
         ok_env (G1 ++ BindVar ty :: G2) ->
-        ok_env (G1 ++ SkipVar :: G2).
+        ok_env (G1 ++ G2).
     Proof. Admitted.
     (*   introv Henv. induction* G1 ; rew_list in *. inverts* Henv. *)
     (*   destruct* a ; inverts* Henv. constructor*. *)
@@ -513,114 +515,57 @@ Module Soundness (P : PAT).
     (*   constructor. apply* IHG1. apply* ok_type_strengthen_var. *)
     (* Qed. *)
 
-    Lemma ok_data_drop_var :
-      forall G1 G2 d,
-        ok_data (G1 ++ SkipVar :: G2) d ->
-        ok_data (G1 ++ G2) d.
-    Proof. Admitted.
-
-    Lemma ok_kind_drop_var :
-      forall G1 G2 k,
-        ok_kind (G1 ++ SkipVar :: G2) k ->
-        ok_kind (G1 ++ G2) k.
-    Proof. Admitted.
-
-    Lemma ok_type_drop_var :
-      forall G1 G2 ty k,
-        ok_type (G1 ++ SkipVar :: G2) ty k ->
-        ok_type (G1 ++ G2) ty k.
-    Proof. Admitted.
-
-    Lemma ok_env_drop_var :
-      forall G1 G2,
-        ok_env (G1 ++ SkipVar :: G2) ->
-        ok_env (G1 ++ G2).
-    Proof. Admitted.
-    (*   introv Henv. induction* G1 ; rew_list in *. inverts* Henv. *)
-    (*   destruct* a ; inverts* Henv. constructor*. *)
-    (*   apply* ok_data_drop_var. apply* ok_type_drop_var. unfolds tnames. rew_listx in *. *)
-    (*   unfold is_tname in *. rew_env* in *. *)
-    (*   constructor. apply* IHG1. apply* ok_kind_drop_var. *)
-    (*   constructor. apply* IHG1. apply* ok_type_drop_var. *)
-    (* Qed. *)
-
     Lemma tm_freshen_preservation :
-      forall Gamma t ty b,
-        is_var b ->
+      forall Gamma t ty ty',
         ok_term Gamma t ty ->
-        ok_term (b :: Gamma) (tm_freshen t 0) ty.
+        ok_term (BindVar ty' :: Gamma) (tm_freshen t 0) ty.
     Proof. Admitted.
 
     Lemma tm_ty_freshen_preservation :
-      forall Gamma t ty b,
-        is_tvar b ->
+      forall Gamma t ty k,
         ok_term Gamma t ty ->
-        ok_term (b :: Gamma) (tm_ty_freshen t 0) ty.
+        ok_term (BindTvar k :: Gamma) (tm_ty_freshen t 0) ty.
     Proof. Admitted.
 
-    Lemma ok_term_drop_var :
-      forall G1 G2 t ty,
-        ok_term (G1 ++ SkipVar :: G2) t ty ->
-        ok_term (G1 ++ G2) (tm_defreshen t (length (vars G1))) ty.
-    Proof.
-      introv ttype.
-      remember (G1 ++ SkipVar :: G2) as Gamma eqn:HGamma.
-      gen G1.
-      induction ttype ; intros ; subst*.
-      { Case "TmFVar". with_hyp (var_in _ _ _) as Hvar. rew_env in Hvar. unfolds var_in.
-        unfold tm_defreshen.
-        lets [ in_vs1 | (m' & Heqm' & in_vs2') ] : Nth_app_inv Hvar.
-        { lets Hlt : Nth_inbound in_vs1. simple_math.
-          constructor. apply* ok_env_drop_var. unfold var_in. rew_env.
-          applys* Nth_app_l. }
-        { lets [ (Heq0 & Heqty) | (m & Heqm & in_vs2) ] : Nth_cons_inv in_vs2' ; subst.
-          { inverts Heqty. }
-          { simple_math. constructor. apply* ok_env_drop_var. unfold var_in. rew_env.
-            applys_eq* (>> Nth_app_r in_vs2). nat_math. } } }
-      { Case "TmLam". constructor. apply* ok_type_drop_var.
-        rewrite tm_open_defreshen_comm.
-        applys_eq* (IHttype (BindVar ty1 :: G1)). rew_env*. }
-      { Case "TmTyLam". constructor. apply* ok_kind_drop_var.
-        rewrite tm_ty_open_defreshen_comm.
-        applys_eq* (IHttype (BindTvar k :: G1)). rew_env*. }
-      { Case "TmTyApp". constructors*. apply* ok_type_drop_var. }
-    Qed.
-
-    Lemma tm_subst_preservation :
-      forall G1 G2 t t' ty1 ty2,
+    Lemma tm_close_preservation :
+      forall G1 G2 x t t' ty1 ty2,
+        x = length (vars G1) ->
         ok_term (G1 ++ BindVar ty1 :: G2) t ty2 ->
-        ok_term (G1 ++ SkipVar :: G2) t' ty1 ->
-        ok_term (G1 ++ SkipVar :: G2) (tm_subst t (length (vars G1)) t') ty2.
+        ok_term (G1 ++ G2) t' ty1 ->
+        ok_term (G1 ++ G2) (tm_close t x t') ty2.
     Proof.
-      introv ttype.
+      introv Heq ttype. unfolds tm_close.
       remember (G1 ++ BindVar ty1 :: G2) as Gamma eqn:HGamma.
-      gen t' G1.
+      gen t' G1 x.
       induction ttype ; intros ; subst*.
-      { Case "TmFVar".
-        with_hyp (var_in _ _ _) as Hvar. rew_env in Hvar. unfolds var_in.
-        unfold tm_subst.
+      { Case "TmFVar". with_hyp (var_in _ _ _) as Hvar. unfolds in Hvar. rew_env in Hvar.
         lets [ in_vs1 | (m' & Heqm' & in_vs2') ] : Nth_app_inv Hvar.
         { lets Hlt : Nth_inbound in_vs1. simple_math.
           constructor. apply* ok_env_strengthen_var. unfold var_in. rew_env.
           applys* Nth_app_l. }
         { lets [ (Heq0 & Heqty) | (m & Heqm & in_vs2) ] : Nth_cons_inv in_vs2'.
-          { inverts* Heqty. simple_math. }
+          { inverts* Heqty. simple_math. rewrite* tm_defreshen_freshen. }
           { simple_math. constructor. apply* ok_env_strengthen_var. unfold var_in. rew_env.
-            applys_eq* (>> Nth_app_r (vars G1 ++ [SkipVar]) in_vs2) ; rew_list~. nat_math. } } }
-      { Case "TmLam". constructor. applys* ok_type_strengthen_var ty1.
-        rewrite tm_open_subst_comm.
+            applys_eq* (>> Nth_app_r (vars G1) in_vs2) ; rew_list~. nat_math. } } }
+      { Case "TmLam". constructor. apply* ok_type_strengthen_var.
+        rewrite tm_open_defreshen_comm. rewrite tm_open_fsubst_comm.
         applys_eq* (IHttype (tm_freshen t' 0) (BindVar ty0 :: G1)). rew_env*.
-        rew_list. applys* tm_freshen_preservation. applys* ok_term_lc. }
-      { Case "TmTyLam". constructor. applys* ok_kind_strengthen_var ty1.
-        rewrite tm_ty_open_subst_comm.
+        rewrite* tm_freshen_freshen. nat_math.
+        rew_list. applys* tm_freshen_preservation.
+        applys* tm_freshen_lc. applys* ok_term_lc. }
+      { Case "TmApp". constructors*. }
+      { Case "TmTyLam". constructor. apply* ok_kind_strengthen_var.
+        rewrite tm_ty_open_defreshen_comm. rewrite tm_ty_open_fsubst_comm.
         applys_eq* (IHttype (tm_ty_freshen t' 0) (BindTvar k :: G1)). rew_env*.
-        rew_list. applys* tm_ty_freshen_preservation. applys* ok_term_lc. }
-      { Case "TmTyApp". constructors*. applys* ok_type_strengthen_var ty1. }
+        rewrite* tm_ty_freshen_freshen.
+        rew_list. applys* tm_ty_freshen_preservation.
+        applys* tm_freshen_lc. applys* ok_term_lc. }
+      { Case "TmTyApp". constructors*. apply* ok_type_strengthen_var. }
     Qed.
 
-    Lemma tm_ty_subst_preservation :
+    Lemma tm_ty_close_preservation :
       forall Gamma t ty ty' k,
-        ok_term (BindTvar k :: Gamma) (tm_ty_open t) (ty_open ty) ->
+        ok_term (BindTvar k :: Gamma) (tm_ty_open t 0 0) (ty_open ty 0 0) ->
         ok_type Gamma ty' k ->
         ok_term Gamma (tm_ty_bsubst t 0 ty') (ty_bsubst ty 0 ty').
     Proof. Admitted.
@@ -636,11 +581,9 @@ Module Soundness (P : PAT).
       induction ttype ; intros ; inverts tstep
       ; try (with_hyp (is_context _) as ctx ; with_hyp (_ = _) as eq
              ; inverts ctx ; inverts* eq).
-      { Case "TmApp". inverts ttype1. rewrite tm_subst_open.
-        applys* ok_term_drop_var empty_env Gamma.
-        applys* tm_subst_preservation empty_env Gamma ty1.
-        applys* tm_freshen_preservation ttype2. }
-      { Case "TmTyApp". inverts ttype. applys* tm_ty_subst_preservation. }
+      { Case "TmApp". inverts ttype1. rewrite tm_bsubst_close_open with (x := 0).
+        applys* tm_close_preservation empty_env Gamma ty1. }
+      { Case "TmTyApp". inverts ttype. applys* tm_ty_close_preservation. }
     Qed.
   End Soundness.
 End Soundness.
